Apply Patch from @kyoDralliam

examples/algorithms/GenericStability.fst
@@ -26,7 +26,7 @@ let rec filter_eq #a x xs k =
       else filter_eq x tl k
 
 val filter_eq_contains: #a:eqtype -> (k:int) -> (xs: list a) -> key:(a -> Tot int) ->
-  Lemma(ensures(forall x. (mem x xs /\ key x = k) <==> mem x (filter_eq k xs key)))
+  Lemma (ensures (forall x. (mem x xs /\ key x = k) <==> mem x (filter_eq k xs key)))
 let rec filter_eq_contains #a k xs key =
   match xs with
   | [] -> ()
@@ -34,7 +34,7 @@ let rec filter_eq_contains #a k xs key =
     filter_eq_contains k tl key
 
 val filter_eq_append: #a:eqtype -> (l1: list a) -> (l2: list a) -> k:(a -> Tot int) ->
-  Lemma(ensures(forall x. (filter_eq x l1 k)@(filter_eq x l2 k) = filter_eq x (l1@l2) k))
+  Lemma (ensures (forall x. (filter_eq x l1 k)@(filter_eq x l2 k) = filter_eq x (l1@l2) k))
 let rec filter_eq_append #a l1 l2 k =
   match l1 with
   | [] -> ()
@@ -42,7 +42,7 @@ let rec filter_eq_append #a l1 l2 k =
     filter_eq_append tl l2 k
 
 val filter_eq_not_contains: #a:eqtype -> (l: list a) -> k:(a -> Tot int) ->
-  Lemma(ensures (forall x. (filter_eq x l k) = [] <==> ~(exists e. (mem e l /\ k e = x))))
+  Lemma (ensures (forall x. (filter_eq x l k) = [] <==> ~(exists e. (mem e l /\ k e = x))))
 let rec filter_eq_not_contains #a l k =
   match l with
   | [] -> ()
@@ -50,24 +50,24 @@ let rec filter_eq_not_contains #a l k =
     filter_eq_not_contains tl k
 
 val filter_eq_single: #a:eqtype ->
-  (l: list a{is_Cons l /\ length l = 1}) ->
+  (l: list a{Cons? l /\ length l = 1}) ->
   k:(a -> Tot int) ->
-  Lemma(ensures(forall x. (k (hd l) = x ) ==> filter_eq x l k = [hd l]))
+  Lemma (ensures (forall x. (k (hd l) = x ) ==> filter_eq x l k = [hd l]))
 let filter_eq_single #a l k = ()
 
-val filter_eq_sorted_lt:  #a:eqtype -> l:list a{is_Cons l} -> k:(a -> Tot int) ->
-  Lemma(requires (sorted l k))
-  (ensures(forall x. (x < k (hd l)) ==> (filter_eq x l k = [])))
+val filter_eq_sorted_lt:  #a:eqtype -> l:list a{Cons? l} -> k:(a -> Tot int) ->
+  Lemma (requires (sorted l k))
+        (ensures (forall x. (x < k (hd l)) ==> (filter_eq x l k = [])))
 let filter_eq_sorted_lt #a l k =
   sorted_lt l k;
   filter_eq_not_contains l k
 
 val filter_eq_first: #a:eqtype ->
-  (l1: list a{is_Cons l1}) ->
-  (l2: list a{is_Cons l2}) ->
+  (l1: list a{Cons? l1}) ->
+  (l2: list a{Cons? l2}) ->
   k:(a -> Tot int) ->
-  Lemma(requires (sorted l1 k) /\  (k (hd l1) > k (hd l2)))
-  (ensures (forall x. (k (hd l2) = x ) ==>
+  Lemma (requires (sorted l1 k) /\  (k (hd l1) > k (hd l2)))
+        (ensures (forall x. (k (hd l2) = x ) ==>
     filter_eq x (l1@l2) k = ((filter_eq x ((hd l2)::l1) k )@(filter_eq x (tl l2) k))))
 let filter_eq_first #a l1 l2 k =
   filter_eq_append l1 l2 k;
@@ -76,11 +76,11 @@ let filter_eq_first #a l1 l2 k =
 type stable (#a:eqtype) (l1:list a) (l2:list a) (k:(a -> Tot int)) = forall x. (filter_eq x l1 k = filter_eq x l2 k)
 
 val stable_lift: #a:eqtype ->
-  (l1: list a{is_Cons l1}) ->
-  (l2: list a{is_Cons l2}) ->
+  (l1: list a{Cons? l1}) ->
+  (l2: list a{Cons? l2}) ->
   k:(a -> Tot int) ->
-  Lemma(requires (sorted l1 k) /\ (k (hd l1) > k (hd l2)))
-  (ensures (stable (l1@l2) (((hd l2)::l1)@(tl l2)) k))
+  Lemma (requires (sorted l1 k) /\ (k (hd l1) > k (hd l2)))
+        (ensures (stable (l1@l2) (((hd l2)::l1)@(tl l2)) k))
 let stable_lift #a l1 l2 k =
   filter_eq_append l1 l2 k;
   filter_eq_append ((hd l2)::l1) (tl l2) k;
@@ -92,7 +92,7 @@ val stable_append_l: #a:eqtype ->
   (r: list a) ->
   (r': list a) ->
   k:(a -> Tot int) ->
-  Lemma(ensures(stable r r' k ==> stable (l@r) (l@r') k))
+  Lemma (ensures (stable r r' k ==> stable (l@r) (l@r') k))
 let rec stable_append_l #a l r r' k =
   match l with
   | [] -> ()
@@ -103,20 +103,20 @@ val stable_append_r: #a:eqtype ->
   (l': list a) ->
   (r: list a) ->
   k:(a -> Tot int) ->
-  Lemma(requires(stable l l' k))
-  (ensures(stable (l@r) (l'@r) k))
+  Lemma (requires (stable l l' k))
+        (ensures(stable (l@r) (l'@r) k))
 let rec stable_append_r #a l l' r k =
   filter_eq_append l r k;
   filter_eq_append l' r k
 
-val stable_commutative: #a:eqtype
+val stable_transitive: #a:eqtype
   -> (l1:list a)
   -> (l2:list a)
   -> (l3:list a)
   -> k:(a -> Tot int)
-  -> Lemma(requires(stable l1 l2 k /\ stable l2 l3 k))
-  (ensures(stable l1 l3 k))
-let stable_commutative #a l1 l2 l3 k = ()
+  -> Lemma (requires (stable l1 l2 k /\ stable l2 l3 k))
+          (ensures (stable l1 l3 k))
+let stable_transitive #a l1 l2 l3 k = ()
 
 val stable_append: #a:eqtype
   -> (l1:list a)
@@ -124,8 +124,8 @@ val stable_append: #a:eqtype
   -> (r1:list a)
   -> (r2:list a)
   -> k:(a -> Tot int)
-  -> Lemma(requires(stable l1 l2 k /\ stable r1 r2 k))
-  (ensures(stable (l1@r1) (l2@r2) k))
+  -> Lemma (requires (stable l1 l2 k /\ stable r1 r2 k))
+          (ensures (stable (l1@r1) (l2@r2) k))
 let stable_append #a l1 l2 r1 r2 k =
   stable_append_r l1 l2 r1 k;
   stable_append_l l2 r1 r2 k
