examples/algorithms/MergeSort2.fst
@@ -19,9 +19,11 @@ val merge': #a:eqtype -> (l1:list a) -> (l2:list a) -> k:(a -> Tot int) -> Tot (
 let rec merge' #a l1 l2 k = match (l1, l2) with
   | [], _ -> l2
   | _, [] -> l1
-  | h1::tl1, h2::tl2 -> if k h1 <= k h2
-                        then h1::(merge' tl1 l2 k)
-                        else h2::(merge' l1 tl2 k)
+  | h1::tl1, h2::tl2 ->
+    if k h1 <= k h2
+    then h1::(merge' tl1 l2 k)
+    else h2::(merge' l1 tl2 k)
+
 (** merging l and r returns a permutation of l and r **)
 val merge'_permutation: #a:eqtype ->
   (l1:list a) ->
@@ -31,25 +33,29 @@ val merge'_permutation: #a:eqtype ->
 let rec merge'_permutation #a l1 l2 k = match (l1, l2) with
   | [], _ -> ()
   | _, [] -> ()
-  | h1::tl1, h2::tl2 -> if k h1 <= k h2
-                          then (merge'_permutation tl1 l2 k)
-                        else (merge'_permutation l1 tl2 k)
+  | h1::tl1, h2::tl2 ->
+    if k h1 <= k h2
+    then (merge'_permutation tl1 l2 k)
+    else (merge'_permutation l1 tl2 k)
+
 (** merging two sorted lists returns a sorted list **)
 val merge'_sorted: #a:eqtype ->
   (l1:list a) ->
   (l2:list a) ->
   k:(a -> Tot int) ->
-  Lemma(requires (sorted l1 k /\ sorted l2 k))
-    (ensures sorted (merge' l1 l2 k) k)
-let rec merge'_sorted #a l1 l2 k =
-match (l1, l2) with
+  Lemma (requires (sorted l1 k /\ sorted l2 k))
+        (ensures sorted (merge' l1 l2 k) k)
+let rec merge'_sorted #a l1 l2 k = match (l1, l2) with
   | [], _ -> ()
   | _, [] -> ()
-  | h1::tl1, h2::tl2 -> if k h1 <= k h2
-                          then (merge'_sorted tl1 l2 k)
-                        else (merge'_sorted l1 tl2 k)
+  | h1::tl1, h2::tl2 ->
+    if k h1 <= k h2
+    then (merge'_sorted tl1 l2 k)
+    else (merge'_sorted l1 tl2 k)
+
 (** This identity for merge is important later **)
-val merge'_hd: #a:eqtype -> l:list a{is_Cons l} -> r:list a{is_Cons r} -> k:(a -> Tot int) ->
+(* KM : Really needed ? *)
+val merge'_hd: #a:eqtype -> l:list a{Cons? l} -> r:list a{Cons? r} -> k:(a -> Tot int) ->
   Lemma(ensures
   ((k (hd l) <= k (hd r)) ==> (merge' l r k = ((hd l)::(merge' (tl l) r k))) /\
   ((k (hd l) > k (hd r)) ==> (merge' l r k = ((hd r)::(merge' l (tl r) k))))))
@@ -65,25 +71,25 @@ val merge'_nil_r: #a:eqtype -> (r: list a) -> k:(a -> Tot int) ->
 let merge'_nil_r #a r k = ()
 
 (** filtering (l appended to r) wrt x is equivelant to merging l and r, then filtering wrt x **)
-val merge'_filter_eq_inv: #a:eqtype -> (l: list a{is_Cons l}) -> (r: list a{is_Cons r}) -> k:(a -> Tot int) ->
-  Lemma(requires (sorted l k /\ sorted r k))
-    (ensures (forall x. ((is_Cons l /\ is_Cons r)/\ (filter_eq x (l@r) k = filter_eq x (merge' l r k) k))))
+val merge'_filter_eq_inv: #a:eqtype -> (l: list a{Cons? l}) -> (r: list a{Cons? r}) -> k:(a -> Tot int) ->
+  Lemma (requires (sorted l k /\ sorted r k))
+        (ensures (forall x. Cons? l /\ Cons? r /\ (filter_eq x (l@r) k = filter_eq x (merge' l r k) k)))
 let rec merge'_filter_eq_inv #a l r k =
   if k (hd r) < k (hd l) then
     (stable_lift l r k;
-    merge'_hd l r k;
-    if (tl r) = [] then merge'_l_nil l k
+    //merge'_hd l r k;
+    if (tl r) = [] then () //merge'_l_nil l k
     else (merge'_filter_eq_inv l (tl r) k;
       filter_eq_append [hd r] (merge' l (tl r) k) k))
-  else (merge'_hd l r k;
-    if (tl l) = [] then (merge'_nil_r r k)
+  else ( //merge'_hd l r k;
+    if (tl l) = [] then () //(merge'_nil_r r k)
     else (merge'_filter_eq_inv (tl l) r k;
       filter_eq_append [hd l] (merge' (tl l) r k) k))
 
 (** merge is stable **)
-val merge'_stable: #a:eqtype -> (l: list a{is_Cons l}) -> (r: list a{is_Cons r}) -> k:(a -> Tot int) ->
-  Lemma(requires (sorted l k /\ sorted r k))
-  (ensures stable (l@r) (merge' l r k) k)
+val merge'_stable: #a:eqtype -> (l: list a{Cons? l}) -> (r: list a{Cons? r}) -> k:(a -> Tot int) ->
+  Lemma (requires (sorted l k /\ sorted r k))
+        (ensures stable (l@r) (merge' l r k) k)
 let merge'_stable #a l r k = merge'_filter_eq_inv l r k
 
 (** split_n splits a list at index n **)
@@ -106,10 +112,11 @@ let split_half #a l = split_n l ((length l) / 2)
 val mergesort': #a:eqtype -> l:list a -> k:(a -> Tot int) -> Tot (l':list a) (decreases (length l))
 let rec mergesort' #a l k =
   match l with
-  | [] | [_] -> l
-  | a::b::tl ->
-    let splt = split_half l in
-    merge' (mergesort' (fst splt) k) (mergesort' (snd splt) k) k
+  | []
+  | [_] -> l
+  | _::_::_ ->
+    let splt1, splt2 = split_half l in
+    merge' (mergesort' splt1 k) (mergesort' splt2 k) k
 
 (** Mergesort returns a sorted list **)
 val mergesort'_sorted: #a:eqtype -> l:list a -> k:(a -> Tot int) ->
@@ -117,12 +124,13 @@ val mergesort'_sorted: #a:eqtype -> l:list a -> k:(a -> Tot int) ->
   (decreases (length l))
 let rec mergesort'_sorted #a l k =
   match l with
-  | [] | [_] -> ()
-  | a::b::tl ->
-    let splt = split_half l in
-    mergesort'_sorted (fst splt) k;
-    mergesort'_sorted (snd splt) k;
-    merge'_sorted (mergesort' (fst splt) k) (mergesort' (snd splt) k) k
+  | []
+  | [_] -> ()
+  | _::_::_ ->
+    let splt1, splt2 = split_half l in
+    mergesort'_sorted splt1 k;
+    mergesort'_sorted splt2 k;
+    merge'_sorted (mergesort' splt1 k) (mergesort' splt2 k) k
 
 (** Mergesort returns a permutation of it's input **)
 val mergesort'_permutation: #a:eqtype -> l:list a -> k:(a -> Tot int) ->
@@ -131,11 +139,11 @@ val mergesort'_permutation: #a:eqtype -> l:list a -> k:(a -> Tot int) ->
 let rec mergesort'_permutation #a l k =
   match l with
   | [] | [_] -> ()
-  | a::b::tl ->
-    let splt = split_half l in
-    mergesort'_permutation (fst splt) k;
-    mergesort'_permutation (snd splt) k;
-    merge'_permutation (mergesort' (fst splt) k) (mergesort' (snd splt) k) k
+  | _::_::_ ->
+    let splt1, splt2 = split_half l in
+    mergesort'_permutation splt1 k;
+    mergesort'_permutation splt2 k;
+    merge'_permutation (mergesort' splt1 k) (mergesort' splt2 k) k
 
 (** Mergesort is stable **)
 val mergesort'_stable: #a:eqtype -> l:list a -> k:(a -> Tot int) ->
@@ -144,14 +152,14 @@ val mergesort'_stable: #a:eqtype -> l:list a -> k:(a -> Tot int) ->
 let rec mergesort'_stable #a l k =
   match l with
   | [] | [_] -> ()
-  | a::b::tl ->
-    let splt = split_half l in
-    mergesort'_stable (fst splt) k;
-    mergesort'_stable (snd splt) k;
-    stable_append (fst splt) (mergesort' (fst splt) k) (snd splt) (mergesort' (snd splt) k) k;
-    mergesort'_sorted (fst splt) k;
-    mergesort'_sorted (snd splt) k;
-    merge'_stable (mergesort' (fst splt) k) (mergesort' (snd splt) k) k
+  | _::_::_ ->
+    let splt1, splt2 = split_half l in
+    mergesort'_stable splt1 k;
+    mergesort'_stable splt2 k;
+    stable_append splt1 (mergesort' splt1 k) splt2 (mergesort' splt2 k) k;
+    mergesort'_sorted splt1 k;
+    mergesort'_sorted splt2 k;
+    merge'_stable (mergesort' splt1 k) (mergesort' splt2 k) k
 
 (** Finally, we define mergesort and prove it's properties**)
 val mergesort: #a:eqtype -> l:list a -> k:(a -> Tot int) ->
